corecursive interface for CompM

Freigen/CompM/Basic.lean
@@ -21,6 +21,85 @@ instance {γ : Γ} : LawfulMonad (CompM E γ) :=
 
 namespace CompM
 
+private def treeEquiv {γ : Γ} {α : Type v} :
+    CompM E γ α ≃ ITree E γ α :=
+  ExactCodensity.equiv
+
+private def actionEquiv
+    {I : Type ui} {O : Type uo}
+    {F : IxPoly I O}
+    {X : I → Type ux} {Y : I → Type uy}
+    (e : (i : I) → X i ≃ Y i)
+    (o : O) :
+    F X o ≃ F Y o where
+  toFun := IxPoly.map (fun i => e i) o
+  invFun := IxPoly.map (fun i => (e i).symm) o
+  left_inv x := by
+    rw [IxPoly.map_map]
+    simpa only [Equiv.symm_apply_apply] using IxPoly.map_id o x
+  right_inv y := by
+    rw [IxPoly.map_map]
+    simpa only [Equiv.apply_symm_apply] using IxPoly.map_id o y
+
+def observe {γ : Γ} {α : Type v} :
+    CompM E γ α ≃
+      Eff.Step Γ E (fun i => CompM E i.1 i.2) (γ, α) :=
+  treeEquiv.trans <|
+    ITree.observe.trans <|
+      actionEquiv (fun _ => treeEquiv.symm) (γ, α)
+
+def roll {γ : Γ} {α : Type v} :
+    Eff.Step Γ E (fun i => CompM E i.1 i.2) (γ, α) →
+      CompM E γ α :=
+  observe.symm
+
+@[simp]
+theorem observe_roll
+    {γ : Γ} {α : Type v}
+    (x : Eff.Step Γ E (fun i => CompM E i.1 i.2) (γ, α)) :
+    observe (roll x) = x :=
+  observe.apply_symm_apply x
+
+@[simp]
+theorem roll_observe
+    {γ : Γ} {α : Type v}
+    (x : CompM E γ α) :
+    roll (observe x) = x :=
+  observe.symm_apply_apply x
+
+def corec
+    {A : Γ × Type v → Type w}
+    (f : (i : Γ × Type v) → A i → Eff.Step Γ E A i)
+    {i : Γ × Type v}
+    (a : A i) :
+    CompM E i.1 i.2 :=
+  treeEquiv.symm (ITree.corec f a)
+
+theorem observe_corec
+    {A : Γ × Type v → Type w}
+    (f : (i : Γ × Type v) → A i → Eff.Step Γ E A i)
+    {i : Γ × Type v}
+    (a : A i) :
+    observe (corec f a) =
+      IxPoly.map
+        (fun _ y => corec f y)
+        i
+        (f i a) := by
+  change
+    IxPoly.map (fun _ x => treeEquiv.symm x) i
+      (ITree.observe
+        (treeEquiv (treeEquiv.symm (ITree.corec f a)))) =
+    IxPoly.map (fun _ y => treeEquiv.symm (ITree.corec f y)) i (f i a)
+  rw [Equiv.apply_symm_apply, ITree.observe_corec]
+  rw [IxPoly.map_map]
+
+theorem eq_of_observe_eq
+    {γ : Γ} {α : Type v}
+    {x y : CompM E γ α}
+    (h : observe x = observe y) :
+    x = y :=
+  observe.injective h
+
 private theorem bind_def
     {γ : Γ} {α β : Type}
     (x : CompM E γ α) (f : α → CompM E γ β) :
